progress in clight gen proof

rustfrontend/Clightgenproof.v
@@ -11,55 +11,171 @@ Require Import Clight.
 Require Import RustlightBase RustIR.
 Require Import Errors.
 Require Import Clightgen.
+Require Import LanguageInterface cklr.CKLR cklr.Inject cklr.InjectFootprint.
 
 Import ListNotations.
 
 (** Correctness proof for the generation of Clight *)
 
+Record match_prog (p: RustIR.program) (tp: Clight.program) : Prop := {
+    match_prog_main:
+    tp.(Ctypes.prog_main) = p.(prog_main);
+    match_prog_public:
+    tp.(Ctypes.prog_public) = p.(prog_public);
+    match_prog_types:
+    tp.(Ctypes.prog_types) = transl_composites p.(prog_types)
+  }.
+
+Section PRESERVATION.
 
 Variable match_prog: RustIR.program -> Clight.program -> Prop. (* TODO *)
 
+Variable prog: RustIR.program.
+Variable tprog: Clight.program.
+Hypothesis TRANSL: match_prog  prog tprog.
 
+Variable se: Genv.symtbl.
+Variable tse: Genv.symtbl.
+(* injp or inj ? *)
+Variable w: world injp.
+Let ge := RustIR.globalenv se prog.
+Let tge := Clight.globalenv tse tprog.
+
+(** TODO: Relational specification of the translation. *)
+
+Variable tr_stmt: composite_env -> Ctypes.composite_env -> PTree.t ident -> RustIR.statement -> Clight.statement -> Prop.
 
 (* Simulation relation *)
 
-Variable ce: composite_env.
-Variable tce: Ctypes.composite_env.
+Let ce := prog.(prog_comp_env).
+Let tce := tprog.(Ctypes.prog_comp_env).
 Variable dropm: PTree.t ident.
-Hypothesis match_composites: composite_env -> Ctypes.composite_env -> Prop.
-
-Inductive match_cont : RustIR.cont -> Clight.cont -> Prop :=
-| match_Kstop: match_cont RustIR.Kstop Clight.Kstop
-| match_Kseq: forall s ts k tk g g',
-    (* To avoid generator, we need to build the spec *)
-    transl_stmt ce tce dropm s g = Res ts g' ->
-    match_cont k tk ->
-    match_cont (RustIR.Kseq s k) (Clight.Kseq ts tk)
-(** TODO  *)
-.
 
 Definition match_env (f: meminj) (e: env) (te: Clight.env) : Prop :=
   (* me_mapped in Simpllocalproof.v *)
   forall id b ty, e!id = Some (b, ty) ->
           exists tb, te!id = Some (tb, to_ctype ty) /\ f b = Some (tb, 0).
-                    
 
-Inductive match_states: RustIR.state -> Clight.state -> Prop :=
-| match_states_regular: forall f tf s ts k tk m tm e te le j g1 g2,
-    (* Ignore the generators here *)
-    transl_function ce tce dropm f = OK tf ->
-    transl_stmt ce tce dropm s g1 = Res ts g2 ->
-    (* match continuation *)
+
+Inductive match_cont : RustIR.cont -> Clight.cont -> Prop :=
+| match_Kstop: match_cont RustIR.Kstop Clight.Kstop
+| match_Kseq: forall s ts k tk,
+    (* To avoid generator, we need to build the spec *)
+    tr_stmt ce tce dropm s ts ->
     match_cont k tk ->
-    (* we need to consider that tm may contains more block for its call of drop glue *)
-    (* use injp_acc ? *)
-    Mem.inject j m tm ->
-    (* local environments are the same? *)
-    match_env j e te ->
-    match_states (RustIR.State f s k e m) (Clight.State tf ts tk te le tm)
-
+    match_cont (RustIR.Kseq s k) (Clight.Kseq ts tk)
+| match_Kloop: forall s ts k tk,
+    tr_stmt ce tce dropm s ts ->
+    match_cont k tk ->
+    match_cont (RustIR.Kloop s k) (Clight.Kloop1 ts Clight.Sskip tk)
+| match_Kcall1: forall p f tf e te le k tk cty temp pe,
+    (* we need to consider temp is set to a Clight expr which is
+    translated from p *)
+    transl_function ce tce dropm f = OK tf ->
+    cty = to_ctype (typeof_place p) ->
+    place_to_cexpr tce p = OK pe ->
+    match_cont k tk ->
+    match_env (mi injp w) e te ->
+    match_cont (RustIR.Kcall (Some p) f e k) (Clight.Kcall (Some temp) tf te le (Clight.Kseq (Clight.Sassign pe (Etempvar temp cty)) tk))
+| match_Kcall2: forall f tf e te le k tk,
+    (* how to relate le? *)
+    transl_function ce tce dropm f = OK tf ->
+    match_cont k tk ->
+    match_cont (RustIR.Kcall None f e k) (Clight.Kcall None tf te le tk)
+| match_Kcalldrop: forall id e te le k tk tf co co_def R,
+    (* Is it correct? *)
+    ce ! id = Some co ->
+    (** TODO  *)
+    R co_def co ->
+    drop_glue_for_composite ce tce dropm co_def = OK (Some tf) ->
+    match_env (mi injp w) e te ->
+    match_cont (RustIR.Kcalldrop id e k) (Clight.Kcall None tf te le tk)
 .
 
+
+Inductive match_states: RustIR.state -> Clight.state -> Prop :=
+| match_regular_state: forall f tf s ts k tk m tm e te le j Hm,
+    (* Ignore the generators here *)
+    transl_function ce tce dropm f = OK tf ->
+    tr_stmt ce tce dropm s ts ->
+    (* match continuation *)
+    match_cont k tk ->
+    (* we need to consider that tm may contains more block for its call stacks of drop glue *)
+    (* use injp_acc ? *)
+    injp_acc w (injpw j m tm Hm) ->
+    (* local environments are the same? *)
+    match_env (mi injp w) e te ->
+    match_states (RustIR.State f s k e m) (Clight.State tf ts tk te le tm)
+| match_call_state: forall vf vargs k m tvf tvargs tk tm j fd targs tres cconv Hm orgs rels
+   (MCONT: match_cont k tk)
+   (VINJ: Val.inject j vf tvf)
+   (MINJ: injp_acc w (injpw j m tm Hm))
+   (AINJ: Val.inject_list j vargs tvargs)
+   (VFIND: Genv.find_funct ge vf = Some fd)
+   (FUNTY: type_of_fundef fd = Tfunction orgs rels targs tres cconv),
+    match_states (RustIR.Callstate vf vargs k m) (Clight.Callstate tvf tvargs tk tm)
+| match_return_state: forall v k m tv tk tm j Hm
+   (MCONT: match_cont k tk)
+   (MINJ: injp_acc w (injpw j m tm Hm))
+   (RINJ: Val.inject j v tv),
+    match_states (RustIR.Returnstate v k m) (Clight.Returnstate tv tk tm)
+| match_calldrop_box: forall p k e m b ofs tk tm ty a j Hm fb
+    (* we can store the address of p in calldrop and build a local env
+    in Drop state according to this address *)
+    (VFIND: Genv.find_def tge fb = Some malloc_decl)
+    (PTY: typeof_place p = Tbox ty a)
+    (PADDR: eval_place ce e m p b ofs)
+    (MCONT: match_cont k tk)
+    (MINJ: injp_acc w (injpw j m tm Hm)),
+    match_states (RustIR.Calldrop p k e m) (Clight.Callstate (Vptr fb Ptrofs.zero) [(Vptr b ofs)] tk tm)
+| match_calldrop_composite: forall p k e m b ofs tk tm a j Hm fb id fid drop_glue orgs
+    (DROPM: dropm!id = Some fid)
+    (VFIND: Genv.find_def tge fb = Some drop_glue)
+    (SYMB: Genv.find_symbol tge fid = Some fb)
+    (* Is it correct? *)
+    (GLUE: In (fid, drop_glue) tprog.(prog_defs))
+    (PTY: typeof_place p = Tstruct orgs id a \/ typeof_place p = Tvariant orgs id a)
+    (PADDR: eval_place ce e m p b ofs)
+    (MCONT: match_cont k tk)
+    (MINJ: injp_acc w (injpw j m tm Hm)),
+    match_states (RustIR.Calldrop p k e m) (Clight.Callstate (Vptr fb Ptrofs.zero) [(Vptr b ofs)] tk tm)
+| match_drop_state: forall id s k e m tf ts tk te le tm j Hm co co_def R
+    (* How to relate e and te? and le? *)
+    (MSTMT: tr_stmt ce tce dropm s ts)
+    (MCONT: match_cont k tk)
+    (MINJ: injp_acc w (injpw j m tm Hm)),
+    ce ! id = Some co ->
+    (** TODO  *)
+    R co_def co ->
+    drop_glue_for_composite ce tce dropm co_def = OK (Some tf) ->
+    match_states (RustIR.Dropstate id s k e m) (Clight.State tf ts tk te le tm)
+.
+
+
+Lemma step_simulation:
+  forall S1 t S2, step ge S1 t S2 ->
+  forall S1' (MS: match_states S1 S1'), exists S2', plus step2 tge S1' t S2' /\ match_states S2 S2'.
+Admitted.
+
+Lemma initial_states_simulation:
+  forall q1 q2 S, match_query (cc_c injp) w q1 q2 -> initial_state ge q1 S ->
+  exists R, Clight.initial_state tge q2 R /\ match_states S R.
+Admitted.
+
+Lemma final_states_simulation:
+  forall S R r1, match_states S R -> final_state S r1 ->
+  exists r2, Clight.final_state R r2 /\ match_reply (cc_c injp) w r1 r2.
+Admitted.
+
+Lemma external_states_simulation:
+  forall S R q1, match_states S R -> at_external ge S q1 ->
+  exists wx q2, Clight.at_external tge R q2 /\ cc_c_query injp wx q1 q2 /\ match_stbls injp wx se tse /\
+  forall r1 r2 S', match_reply (cc_c injp) wx r1 r2 -> after_external S r1 S' ->
+  exists R', Clight.after_external R r2 R' /\ match_states S' R'.
+Admitted.
+
+
+End PRESERVATION.
 
 Theorem transl_program_correct prog tprog:
   match_prog prog tprog ->
